fix compilation (simp more proofs)

Clean/Tables/BLAKE3/ProcessBlocksInductive.lean
@@ -80,11 +80,7 @@ def circuit : FormalAssertion (F p) ProcessBlocksState where
   main
   localLength_eq := by
     simp only [circuit_norm, main, U32.AssertNormalized.circuit]
-  localAdds_eq _ _ _ := by
-    simp only [main, circuit_norm, Operations.localAdds, List.append_nil]
-    apply InteractionDelta.toFinsupp_zero_of_eq_zero
-    apply Circuit.localAdds_forEach
-    intro x n; simp only [circuit_norm, Operations.localAdds]
+  localAdds_eq _ _ _ := by simp only [main, circuit_norm]
   subcircuitsConsistent := by
     simp only [circuit_norm, main, U32.AssertNormalized.circuit]
     omega
@@ -144,11 +140,7 @@ def circuit : FormalAssertion (F p) BlockInput where
   main
   localLength_eq := by
     simp only [circuit_norm, main, U32.AssertNormalized.circuit]
-  localAdds_eq _ _ _ := by
-    simp only [main, circuit_norm, Operations.localAdds]
-    apply InteractionDelta.toFinsupp_zero_of_eq_zero
-    apply Circuit.localAdds_forEach
-    intro x n; simp only [circuit_norm, Operations.localAdds]
+  localAdds_eq _ _ _ := by simp only [main, circuit_norm]
   subcircuitsConsistent := by
     simp only [circuit_norm, main, U32.AssertNormalized.circuit]
   Assumptions _ := True
