Clean/Gadgets/Bits.lean
@@ -26,12 +26,7 @@ def toBits (n : ℕ) (hn : 2^n < p) : GeneralFormalCircuit (F p) field (fields n
   output _ i := varFromOffset (fields n) i
 
   localLength_eq _ _ := by simp only [main, circuit_norm]; ac_rfl
-  localAdds_eq input env offset := by
-    have : (main n input |>.operations offset).localAdds env = 0 := by
-      simp only [main, circuit_norm, Operations.localAdds, List.append_nil, InteractionDelta.zero_eq_nil]
-      apply Circuit.localAdds_forEach
-      intro x n; simp only [circuit_norm, Operations.localAdds]
-    simp only [this, InteractionDelta.toFinsupp_zero]
+  localAdds_eq input offset env := by simp only [main, circuit_norm]
   subcircuitsConsistent x i0 := by simp +arith only [main, circuit_norm]
     -- TODO arith is needed because forAll passes `localLength + offset` while bind passes `offset + localLength`
 
