Clean/Gadgets/Keccak/KeccakState.lean
@@ -71,16 +71,11 @@ lemma KeccakRow.normalized_value_ext (row : KeccakRow (F p)) (rhs : Vector ℕ 5
 -- circuits
 
 def KeccakBlock.normalized : FormalAssertion (F p) KeccakBlock where
-  main block := .forEach block (assertion U64.AssertNormalized.circuit)
+  main block := .forEach block U64.AssertNormalized.circuit
   Assumptions _ := True
   Spec block := block.Normalized
   localLength_eq _ _ := by simp +arith only [circuit_norm, U64.AssertNormalized.circuit]
-  localAdds_eq := by
-    intro block env offset
-    simp only [circuit_norm]
-    apply InteractionDelta.toFinsupp_zero_of_eq_zero
-    apply Circuit.localAdds_forEach
-    intro x n; simp only [circuit_norm, Operations.localAdds]
+  localAdds_eq := by simp only [circuit_norm]
   soundness := by
     simp only [circuit_norm, U64.AssertNormalized.circuit]
     simp [getElem_eval_vector, KeccakBlock.Normalized]
